refactor

.CoqMakefile.d
@@ -1,6 +1,6 @@
 theories/ZPoints.vo theories/ZPoints.glob theories/ZPoints.v.beautified theories/ZPoints.required_vo: theories/ZPoints.v 
 theories/ZPoints.vio: theories/ZPoints.v 
 theories/ZPoints.vos theories/ZPoints.vok theories/ZPoints.required_vos: theories/ZPoints.v 
-theories/Jarvis_March.vo theories/Jarvis_March.glob theories/Jarvis_March.v.beautified theories/Jarvis_March.required_vo: theories/Jarvis_March.v theories/ZPoints.vo
-theories/Jarvis_March.vio: theories/Jarvis_March.v theories/ZPoints.vio
-theories/Jarvis_March.vos theories/Jarvis_March.vok theories/Jarvis_March.required_vos: theories/Jarvis_March.v theories/ZPoints.vos
+theories/Graham_Scan.vo theories/Graham_Scan.glob theories/Graham_Scan.v.beautified theories/Graham_Scan.required_vo: theories/Graham_Scan.v theories/ZPoints.vo
+theories/Graham_Scan.vio: theories/Graham_Scan.v theories/ZPoints.vio
+theories/Graham_Scan.vos theories/Graham_Scan.vok theories/Graham_Scan.required_vos: theories/Graham_Scan.v theories/ZPoints.vos
